bound/LowerBoundExtra.v
@@ -5,7 +5,7 @@ Require Import Locations Stacklayout Conventions Linking.
 Require Export Asm.
 Require Import Simulation Memory ValuesC.
 Require Import Skeleton ModSem Mod sflib AsmC Sem Syntax LinkingC Program SemProps.
-Require Import GlobalenvsC Lia LinkingC2 Conventions1C.
+Require Import GlobalenvsC Lia LinkingC2 Conventions1C JunkBlock StoreArguments.
 
 Set Implicit Arguments.
 
@@ -14,8 +14,238 @@ Local Opaque Z.mul.
 Local Notation "a # b" := (PMap.get b a) (at level 1).
 Local Ltac simp := repeat (bsimpl; des; des_sumbool; ss; clarify).
 
-Existing Instance Val.mi_final.
+Require Import Coq.Classes.RelationClasses.
 
+Inductive inj_same (j: meminj) v0 v1 : Prop :=
+| inj_same_ptr
+    blk0 blk1 blk delta0 delta1 ofs0 ofs1
+    (VAL0: v0 = Vptr blk0 ofs0)
+    (VAL1: v1 = Vptr blk1 ofs1)
+    (INJ0: j blk0 = Some (blk, delta0))
+    (INJ1: j blk1 = Some (blk, delta1))
+    (DELTA: Ptrofs.unsigned ofs0 + delta0 = Ptrofs.unsigned ofs1 + delta1)
+| inj_same_refl
+    (EQ: v0 = v1)
+.
+Hint Constructors inj_same.
+
+Program Instance inj_same_equivalence j: Equivalence (inj_same j).
+Next Obligation. ii. inv H; eauto. Qed.
+Next Obligation.
+  ii. inv H; inv H0; eauto.
+  inv VAL0. rewrite INJ1 in *. inv INJ2. econs; eauto. etrans; eauto.
+Qed.
+
+Lemma inj_same_inj j v0 v1 v_tgt
+      (SAME: inj_same j v0 v1)
+      (INJ: Val.inject j v1 v_tgt)
+  :
+    Val.inject j v0 v_tgt.
+Proof.
+  inv SAME; eauto. inv INJ. rewrite H1 in *. inv INJ1.
+  econs; eauto.
+  erewrite <- (Ptrofs.repr_unsigned ofs1).
+  erewrite <- (Ptrofs.repr_unsigned ofs0).
+  repeat rewrite IntegersC.Ptrofs_add_repr.
+  f_equal. auto.
+Qed.
+
+Lemma inj_same_incr j0 j1
+      (INCR: inject_incr j0 j1)
+  :
+    inj_same j0 <2= inj_same j1.
+Proof.
+  ii. inv PR; eauto.
+Qed.
+
+Lemma separated_out_of_reach j0 j1 m_src0 m_src1 m_tgt0 blk delta
+      (INJ: Mem.inject j0 m_src0 m_tgt0)
+      (INCR: inject_incr j0 j1)
+      (SEPARATED: inject_separated j0 j1 m_src0 m_tgt0)
+      (BOUND: Plt blk m_tgt0.(Mem.nextblock))
+      (OUTOFREACH: loc_out_of_reach j0 m_src0 blk delta)
+      (MAXPERM: forall b ofs p
+                       (VALED: Mem.valid_block m_src0 b)
+                       (PERM: Mem.perm m_src1 b ofs Max p),
+          Mem.perm m_src0 b ofs Max p)
+  :
+    loc_out_of_reach j1 m_src1 blk delta.
+Proof.
+  ii.
+  unfold inject_separated in *.
+  destruct (j0 b0) eqn:EQ.
+  - destruct p. specialize (INCR _ _ _ EQ). clarify.
+    eapply OUTOFREACH; eauto. eapply MAXPERM; eauto.
+    apply NNPP. intro N.
+    eapply Mem.mi_freeblocks in N; eauto. clarify.
+  - specialize (SEPARATED _ _ _ EQ H). des.
+    apply SEPARATED0. eauto.
+Qed.
+
+Lemma unfree_nextblock m_src0 m_src1 blk_src lo hi
+      (UNFREE: Mem_unfree m_src0 blk_src lo hi = Some m_src1)
+  :
+    m_src0.(Mem.nextblock) = m_src1.(Mem.nextblock).
+Proof.
+  unfold Mem_unfree in *. des_ifs.
+Qed.
+
+Record freed_from m0 m1 blk lo hi : Prop :=
+  mk_freed_from
+    {
+      freed_from_unchanged: Mem.unchanged_on
+                              (fun blk' ofs =>
+                                 if eq_block blk' blk
+                                 then ~ (lo <= ofs < hi)
+                                 else True)
+                              m0 m1;
+      freed_from_nextblock: m1.(Mem.nextblock) = m0.(Mem.nextblock);
+      freed_from_perm: Mem.range_perm m0 blk lo hi Cur Freeable;
+      freed_from_noperm: Mem_range_noperm m1 blk lo hi;
+      freed_from_contents: forall ofs (IN: lo <= ofs < hi),
+          ZMap.get ofs (Mem.mem_contents m0) !! blk =
+          ZMap.get ofs (Mem.mem_contents m1) !! blk;
+    }.
+
+Lemma freed_from_perm_le m_src0 m_src1 blk lo hi blk' ofs k p
+      (FREED: freed_from m_src0 m_src1 blk lo hi)
+      (PERM: Mem.perm m_src1 blk' ofs k p)
+  :
+    Mem.perm m_src0 blk' ofs k p.
+Proof.
+  destruct (eq_block blk' blk).
+  - clarify. destruct (classic (lo <= ofs < hi)).
+    + exfalso. eapply freed_from_noperm; eauto.
+      eapply Mem.perm_max. eapply Mem.perm_implies; eauto. econs.
+    + eapply (Mem.unchanged_on_perm _ _ _ (freed_from_unchanged FREED)); auto.
+      des_ifs; eauto.
+      eapply Mem.perm_valid_block in PERM.
+      unfold Mem.valid_block in *. erewrite <- freed_from_nextblock; eauto.
+  - eapply (Mem.unchanged_on_perm _ _ _ (freed_from_unchanged FREED)); auto.
+    des_ifs; eauto.
+    eapply Mem.perm_valid_block in PERM.
+    unfold Mem.valid_block in *. erewrite <- freed_from_nextblock; eauto.
+Qed.
+
+Lemma freed_from_inject j m_src0 m_src1 m_tgt blk lo hi
+      (INJ: Mem.inject j m_src0 m_tgt)
+      (FREED: freed_from m_src0 m_src1 blk lo hi)
+  :
+    Mem.inject j m_src1 m_tgt.
+Proof.
+  eapply Mem.extends_inject_compose; eauto.
+  econs.
+  - eapply freed_from_nextblock; eauto.
+  - econs; i; unfold inject_id in *; clarify; try rewrite Z.add_0_r.
+    + eapply freed_from_perm_le; eauto.
+    + eapply Z.divide_0_r.
+    + destruct (eq_block b2 blk).
+      * clarify. destruct (classic (lo <= ofs < hi)).
+        -- erewrite <- freed_from_contents; eauto. refl.
+        -- erewrite (Mem.unchanged_on_contents _ _ _ (freed_from_unchanged FREED)); auto.
+           refl.
+           des_ifs; eauto.
+           eapply freed_from_perm_le; eauto.
+      * erewrite (Mem.unchanged_on_contents _ _ _ (freed_from_unchanged FREED)); auto.
+        refl.
+        des_ifs; eauto.
+        eapply freed_from_perm_le; eauto.
+  - i. destruct (eq_block b blk).
+    + clarify. destruct (classic (lo <= ofs < hi)).
+      * right. eapply freed_from_noperm; eauto.
+      * left.
+        eapply (Mem.unchanged_on_perm _ _ _ (freed_from_unchanged FREED)); auto.
+        des_ifs; eauto. eapply Mem.perm_valid_block; eauto.
+    + left.
+      eapply (Mem.unchanged_on_perm _ _ _ (freed_from_unchanged FREED)); auto.
+      des_ifs; eauto. eapply Mem.perm_valid_block; eauto.
+Qed.
+
+Lemma freed_from_out_of_reach j m_src0 m_src1 m_tgt blk lo hi blk' delta ofs
+      (INJECT: Mem.inject j m_src0 m_tgt)
+      (FREED: freed_from m_src0 m_src1 blk lo hi)
+      (DELTA: j blk = Some (blk', delta))
+      (IN: lo + delta <= ofs < hi + delta)
+  :
+    loc_out_of_reach j m_src1 blk' ofs.
+Proof.
+  ii. destruct (eq_block b0 blk).
+  - clarify. eapply freed_from_noperm; eauto. omega.
+  - exploit Mem.inject_no_overlap; eauto.
+    + eapply freed_from_perm_le; eauto.
+    + eapply Mem.perm_cur.
+      eapply Mem.perm_implies.
+      eapply freed_from_perm; eauto.
+      instantiate (1 := ofs - delta). omega. econs.
+    + i. des; eauto. omega.
+Qed.
+
+Lemma freed_from_perm_greater m0 m1 blk lo hi
+      (FREE: freed_from m0 m1 blk lo hi)
+  :
+    Mem.perm m1 <4= Mem.perm m0.
+Proof.
+  ii. inv FREE. inv freed_from_unchanged0.
+  specialize (unchanged_on_perm x0 x1 x2 x3).
+  des_ifs; [destruct (zle lo x1); destruct (zlt x1 hi)|];
+    [exploit freed_from_perm0; eauto;
+     i; eapply Mem.perm_cur;
+     eapply Mem.perm_implies; eauto; econs | ..];
+    eapply unchanged_on_perm; eauto with lia;
+      eapply Mem.perm_valid_block in PR; ii;
+        unfold Mem.valid_block; rewrite <- freed_from_nextblock0; auto.
+Qed.
+
+Lemma free_freed_from m0 m1 blk lo hi
+      (FREE: Mem.free m0 blk lo hi = Some m1)
+  :
+    freed_from m0 m1 blk lo hi.
+Proof.
+  econs.
+  - eapply Mem.free_unchanged_on; eauto.
+    i. des_ifs.
+  - eapply Mem.nextblock_free; eauto.
+  - eapply Mem.free_range_perm; eauto.
+  - eapply Mem_free_noperm; eauto.
+  - i. Local Transparent Mem.free. unfold Mem.free in *.
+    des_ifs.
+Qed.
+
+Lemma init_mem_freed_from m_init
+  :
+    freed_from m_init m_init 1%positive 0 0.
+Proof.
+  econs; ii; auto; try omega.
+  econs; eauto. refl.
+Qed.
+
+Inductive skenv_inject {F V} (ge: Genv.t F V) (j: meminj) (m: mem) : Prop :=
+| sken_inject_intro
+    (DOMAIN: forall b, Plt b ge.(Genv.genv_next) -> j b = Some(b, 0))
+    (IMAGE: forall b1 b2 delta (INJ: j b1 = Some(b2, delta))
+                   (PERM: Senv.block_is_volatile ge b1 = true \/ exists ofs, Mem.perm m b1 ofs Max Nonempty),
+        Senv.block_is_volatile ge b2 = Senv.block_is_volatile ge b1)
+.
+
+Lemma skenv_inject_max_perm {F V} (genv: Genv.t F V) (j: meminj) (m0 m1 m_tgt: mem)
+      (INJ: Mem.inject j m0 m_tgt)
+      (MAXPERM: forall b ofs p (VALID: Mem.valid_block m0 b) (PERM: Mem.perm m1 b ofs Max p),
+          Mem.perm m0 b ofs Max p)
+      (SYMB: skenv_inject genv j m0)
+  :
+    skenv_inject genv j m1.
+Proof.
+  inv SYMB. econs; eauto. i. eapply IMAGE; eauto.    
+  unfold symbols_inject_weak in *. des. splits; auto.
+  right. exists ofs. eapply MAXPERM; eauto.
+  eapply Mem.valid_block_inject_1; eauto.
+Qed.
+
+Section INJRANGEWF.
+
+Variable F V: Type.
+Variable ge: Genv.t F V.
+  
 Inductive inj_range_block_wf (j: meminj) (m: mem) blk_src
           (P: Z -> Prop) : Prop :=
 | inj_range_wf_empty
@@ -29,6 +259,10 @@ Inductive inj_range_block_wf (j: meminj) (m: mem) blk_src
         (P (Ptrofs.unsigned ofs) \/
          P (Ptrofs.unsigned ofs - 1) ->
          delta >= 0 /\ 0 <= Ptrofs.unsigned ofs + delta <= Ptrofs.max_unsigned))
+    (VOLATILE: forall
+        ofs
+        (VOL: Senv.block_is_volatile ge blk_src = false)
+        (IN: P ofs), Senv.block_is_volatile ge blk_tgt = Senv.block_is_volatile ge blk_src)
 .
 
 Definition inj_range_wf (j: meminj) (m: mem) (P: Values.block -> Z -> Prop) :=
@@ -45,6 +279,33 @@ Proof.
   - econs 2; eauto; ii.
     + eapply ALIGN. ii. eapply H in PR. des; eauto.
     + eapply RANGE. des; eauto.
+Qed.
+
+Lemma private_unfree_symbols_inject
+      P j m_src0 m_src1 m_tgt blk_src blk_tgt delta lo hi
+      (INJ: Mem.inject j m_src0 m_tgt)
+      (DELTA: j blk_src = Some (blk_tgt, delta))
+      (PERM: Mem.range_perm m_tgt blk_tgt (delta + lo) (delta + hi) Cur Freeable)
+      (UNFREE: Mem_unfree m_src0 blk_src lo hi = Some m_src1)
+      (SYMB: skenv_inject ge j m_src0)
+      (* --------------------------------------------------------- *)
+      (WFINJ: inj_range_wf j m_src0 P)
+      (RANGE: range lo hi <1= P blk_src)
+  :
+    <<SYMB: skenv_inject ge j m_src1>>
+.
+Proof.
+  inv SYMB. econs; auto. i.
+  destruct (WFINJ b1); clarify. des.
+  - exploit IMAGE; eauto.
+  - destruct (classic (brange blk_src lo hi b1 ofs)).
+    + destruct (Senv.block_is_volatile ge b1) eqn:VEQ.
+      * exploit IMAGE; eauto.
+      * unfold brange in *. des. clarify.
+        exploit VOLATILE; eauto.
+    + exploit IMAGE; eauto. right. exists ofs.
+      eapply Mem.unchanged_on_perm; try apply Mem_unfree_unchanged_on; eauto.
+      eapply Mem.valid_block_inject_1; eauto.
 Qed.
 
 Lemma private_unfree_inj_wf
@@ -198,452 +459,21 @@ Lemma private_unfree_inj_inj_wf
       (PERM: Mem.range_perm m_tgt blk_tgt (delta + lo) (delta + hi) Cur Freeable)
       (PRVT: range (delta + lo) (delta + hi) <1= loc_out_of_reach j m_src0 blk_tgt)
       (UNFREE: Mem_unfree m_src0 blk_src lo hi = Some m_src1)
+      (SYMB: skenv_inject ge j m_src0)
       (* --------------------------------------------------------- *)
       (WFINJ: inj_range_wf j m_src0 P)
       (RANGE: range lo hi <1= P blk_src)
   :
-    <<INJ: Mem.inject j m_src1 m_tgt>> /\ <<WFINJ: inj_range_wf j m_src1 P>>
+    (<<INJ: Mem.inject j m_src1 m_tgt>>) /\
+    (<<WFINJ: inj_range_wf j m_src1 P>>) /\
+    (<<SYMB: skenv_inject ge j m_src1>>)
 .
 Proof.
-  split.
+  splits.
   - eapply private_unfree_inj; eauto.
   - eapply private_unfree_inj_wf; eauto.
+  - eapply private_unfree_symbols_inject; eauto.
 Qed.
-
-Lemma separated_out_of_reach j0 j1 m_src0 m_src1 m_tgt0 blk delta
-      (INJ: Mem.inject j0 m_src0 m_tgt0)
-      (INCR: inject_incr j0 j1)
-      (SEPARATED: inject_separated j0 j1 m_src0 m_tgt0)
-      (BOUND: Plt blk m_tgt0.(Mem.nextblock))
-      (OUTOFREACH: loc_out_of_reach j0 m_src0 blk delta)
-      (MAXPERM: forall b ofs p
-                       (VALED: Mem.valid_block m_src0 b)
-                       (PERM: Mem.perm m_src1 b ofs Max p),
-          Mem.perm m_src0 b ofs Max p)
-  :
-    loc_out_of_reach j1 m_src1 blk delta.
-Proof.
-  ii.
-  unfold inject_separated in *.
-  destruct (j0 b0) eqn:EQ.
-  - destruct p. specialize (INCR _ _ _ EQ). clarify.
-    eapply OUTOFREACH; eauto. eapply MAXPERM; eauto.
-    apply NNPP. intro N.
-    eapply Mem.mi_freeblocks in N; eauto. clarify.
-  - specialize (SEPARATED _ _ _ EQ H). des.
-    apply SEPARATED0. eauto.
-Qed.
-
-Program Definition memcpy (m: mem) (blk_old blk_new : Values.block) : mem :=
-  Mem.mkmem
-    (PMap.set blk_new (PMap.get blk_old m.(Mem.mem_contents))
-              m.(Mem.mem_contents))
-    m.(Mem.mem_access) m.(Mem.nextblock)
-                           m.(Mem.access_max) m.(Mem.nextblock_noaccess) _.
-Next Obligation.
-  rewrite PMap.gsspec. des_ifs; apply Mem.contents_default.
-Qed.
-
-Lemma unfree_nextblock m_src0 m_src1 blk_src lo hi
-      (UNFREE: Mem_unfree m_src0 blk_src lo hi = Some m_src1)
-  :
-    m_src0.(Mem.nextblock) = m_src1.(Mem.nextblock).
-Proof.
-  unfold Mem_unfree in *. des_ifs.
-Qed.
-
-Record freed_from m0 m1 blk lo hi : Prop :=
-  mk_freed_from
-    {
-      freed_from_unchanged: Mem.unchanged_on
-                              (fun blk' ofs =>
-                                 if eq_block blk' blk
-                                 then ~ (lo <= ofs < hi)
-                                 else True)
-                              m0 m1;
-      freed_from_nextblock: m1.(Mem.nextblock) = m0.(Mem.nextblock);
-      freed_from_perm: Mem.range_perm m0 blk lo hi Cur Freeable;
-      freed_from_noperm: Mem_range_noperm m1 blk lo hi;
-      freed_from_contents: forall ofs (IN: lo <= ofs < hi),
-          ZMap.get ofs (Mem.mem_contents m0) !! blk =
-          ZMap.get ofs (Mem.mem_contents m1) !! blk;
-    }.
-
-Lemma freed_from_perm_le m_src0 m_src1 blk lo hi blk' ofs k p
-      (FREED: freed_from m_src0 m_src1 blk lo hi)
-      (PERM: Mem.perm m_src1 blk' ofs k p)
-  :
-    Mem.perm m_src0 blk' ofs k p.
-Proof.
-  destruct (eq_block blk' blk).
-  - clarify. destruct (classic (lo <= ofs < hi)).
-    + exfalso. eapply freed_from_noperm; eauto.
-      eapply Mem.perm_max. eapply Mem.perm_implies; eauto. econs.
-    + eapply (Mem.unchanged_on_perm _ _ _ (freed_from_unchanged FREED)); auto.
-      des_ifs; eauto.
-      eapply Mem.perm_valid_block in PERM.
-      unfold Mem.valid_block in *. erewrite <- freed_from_nextblock; eauto.
-  - eapply (Mem.unchanged_on_perm _ _ _ (freed_from_unchanged FREED)); auto.
-    des_ifs; eauto.
-    eapply Mem.perm_valid_block in PERM.
-    unfold Mem.valid_block in *. erewrite <- freed_from_nextblock; eauto.
-Qed.
-
-Lemma freed_from_inject j m_src0 m_src1 m_tgt blk lo hi
-      (INJ: Mem.inject j m_src0 m_tgt)
-      (FREED: freed_from m_src0 m_src1 blk lo hi)
-  :
-    Mem.inject j m_src1 m_tgt.
-Proof.
-  eapply Mem.extends_inject_compose; eauto.
-  econs.
-  - eapply freed_from_nextblock; eauto.
-  - econs; i; unfold inject_id in *; clarify; try rewrite Z.add_0_r.
-    + eapply freed_from_perm_le; eauto.
-    + eapply Z.divide_0_r.
-    + destruct (eq_block b2 blk).
-      * clarify. destruct (classic (lo <= ofs < hi)).
-        -- erewrite <- freed_from_contents; eauto. refl.
-        -- erewrite (Mem.unchanged_on_contents _ _ _ (freed_from_unchanged FREED)); auto.
-           refl.
-           des_ifs; eauto.
-           eapply freed_from_perm_le; eauto.
-      * erewrite (Mem.unchanged_on_contents _ _ _ (freed_from_unchanged FREED)); auto.
-        refl.
-        des_ifs; eauto.
-        eapply freed_from_perm_le; eauto.
-  - i. destruct (eq_block b blk).
-    + clarify. destruct (classic (lo <= ofs < hi)).
-      * right. eapply freed_from_noperm; eauto.
-      * left.
-        eapply (Mem.unchanged_on_perm _ _ _ (freed_from_unchanged FREED)); auto.
-        des_ifs; eauto. eapply Mem.perm_valid_block; eauto.
-    + left.
-      eapply (Mem.unchanged_on_perm _ _ _ (freed_from_unchanged FREED)); auto.
-      des_ifs; eauto. eapply Mem.perm_valid_block; eauto.
-Qed.
-
-Lemma freed_from_out_of_reach j m_src0 m_src1 m_tgt blk lo hi blk' delta ofs
-      (INJECT: Mem.inject j m_src0 m_tgt)
-      (FREED: freed_from m_src0 m_src1 blk lo hi)
-      (DELTA: j blk = Some (blk', delta))
-      (IN: lo + delta <= ofs < hi + delta)
-  :
-    loc_out_of_reach j m_src1 blk' ofs.
-Proof.
-  ii. destruct (eq_block b0 blk).
-  - clarify. eapply freed_from_noperm; eauto. omega.
-  - exploit Mem.inject_no_overlap; eauto.
-    + eapply freed_from_perm_le; eauto.
-    + eapply Mem.perm_cur.
-      eapply Mem.perm_implies.
-      eapply freed_from_perm; eauto.
-      instantiate (1 := ofs - delta). omega. econs.
-    + i. des; eauto. omega.
-Qed.
-
-Definition callee_injection (j: meminj) old_blk new_blk: meminj :=
-  fun blk => if (eq_block blk new_blk)
-             then j old_blk
-             else (j blk).
-
-Lemma freed_from_perm_greater m0 m1 blk lo hi
-      (FREE: freed_from m0 m1 blk lo hi)
-  :
-    Mem.perm m1 <4= Mem.perm m0.
-Proof.
-  ii. inv FREE. inv freed_from_unchanged0.
-  specialize (unchanged_on_perm x0 x1 x2 x3).
-  des_ifs; [destruct (zle lo x1); destruct (zlt x1 hi)|];
-    [exploit freed_from_perm0; eauto;
-     i; eapply Mem.perm_cur;
-     eapply Mem.perm_implies; eauto; econs | ..];
-    eapply unchanged_on_perm; eauto with lia;
-      eapply Mem.perm_valid_block in PR; ii;
-        unfold Mem.valid_block; rewrite <- freed_from_nextblock0; auto.
-Qed.
-
-Local Transparent Mem.alloc.
-Lemma memcpy_inject
-      j m_src0 m_src1 m_src2 m_tgt blk_old blk_new lo hi
-      (INJ: Mem.inject j m_src0 m_tgt)
-      (NEQ: blk_old <> blk_new)
-      (FREE: freed_from m_src0 m_src1 blk_old lo hi)
-      (ALLOC: Mem.alloc m_src1 lo hi = (m_src2, blk_new))
-      blk_tgt delta
-      (INJBLK: j blk_old = Some (blk_tgt, delta))
-  :
-    Mem.inject (callee_injection j blk_old blk_new)
-               (memcpy m_src2 blk_old blk_new) m_tgt
-.
-Proof.
-  assert(JEMPTY: j blk_new = None).
-  { eapply Mem.mi_freeblocks; eauto. unfold Mem.valid_block. erewrite <- freed_from_nextblock; eauto.
-    ii.
-    exploit Mem.alloc_result; eauto. i. clarify. xomega.
-  }
-  assert(INCR: inject_incr j (callee_injection j blk_old blk_new)).
-  { ii; ss. unfold callee_injection. des_ifs. }
-  assert(PERM: Mem.range_perm m_tgt blk_tgt (delta + lo) (delta + hi) Cur Freeable).
-  { clear - INJBLK INJ FREE. ii.
-    assert(exists ofs', ofs = ofs' + delta).
-    { exists (ofs - delta). xomega. } des. clarify.
-    eapply Mem.mi_perm; try apply INJ; try apply INJBLK; eauto.
-    eapply freed_from_perm; eauto. xomega.
-  }
-  unfold callee_injection, memcpy in *.
-  dup INJ.
-  inv INJ.
-  econs; eauto.
-  - clear_until mi_inj.
-    inv mi_inj.
-    econs.
-    + ii; ss.
-      unfold Mem.perm in *. ss.
-      des_ifs.
-      { eapply Mem.perm_cur.
-        eapply Mem.perm_implies with Freeable; try eauto with mem.
-        eapply PERM.
-        exploit Mem.perm_alloc_3; eauto. i.
-        xomega.
-      }
-      destruct (peq b1 blk_old); clarify.
-      { assert(~lo <= ofs < hi).
-        { ii.
-          exploit freed_from_noperm; eauto.
-          eauto with mem.
-        }
-        assert(PERM0: Mem.perm_order' ((Mem.mem_access m_src1) !! blk_old ofs k) p).
-        { eapply Mem.perm_alloc_4; eauto. }
-        eapply mi_perm; eauto.
-        inv FREE.
-        eapply Mem.unchanged_on_perm; eauto.
-        - ii; ss. des_ifs.
-        - apply NNPP. ii. exploit Mem.mi_freeblocks; eauto. i; clarify.
-      }
-      eapply mi_perm; eauto.
-      assert(PERM0: Mem.perm_order' ((Mem.mem_access m_src1) !! b1 ofs k) p).
-      { eapply Mem.perm_alloc_4; eauto. }
-      inv FREE.
-      eapply Mem.unchanged_on_perm; eauto.
-      * ii; ss. des_ifs.
-      * apply NNPP. ii. exploit Mem.mi_freeblocks; eauto. i; clarify.
-    + ii; ss.
-      dup FREE. inv FREE. inv freed_from_unchanged0.
-      des_ifs.
-      * eapply mi_align. eauto. instantiate (2 := ofs). ii.
-        assert (Mem.range_perm m_src2 blk_new ofs (ofs+size_chunk chunk) Max p); eauto.
-        assert (range ofs (ofs + size_chunk chunk) <1= range lo hi).
-        { ii. ii. eapply H2 in PR.
-          eapply Mem.perm_alloc_3 in PR; eauto. }
-        apply H3 in H1. eapply freed_from_perm0 in H1.
-        eapply Mem.perm_cur_max. eauto.
-      * eapply mi_align. eauto. instantiate (2 := ofs).
-        eassert (Mem.range_perm m_src2 b1 ofs (ofs+size_chunk chunk) Max p); eauto.
-        eassert (Mem.range_perm m_src1 b1 ofs (ofs+size_chunk chunk) Max p); eauto.
-        { ii. eapply Mem.perm_alloc_4; eauto. }
-        ii. eapply freed_from_perm_greater; eauto.
-    + ii; ss. rewrite PMap.gsspec. des_ifs.
-      { specialize (mi_memval _ ofs _ _ H).
-        unfold Mem.perm in *. ss.
-        exploit Mem.perm_alloc_3; eauto. i.
-        hexploit1 mi_memval.
-        { eapply Mem.perm_implies with Freeable; eauto with mem.
-          eapply freed_from_perm; eauto.
-        }
-        eapply memval_lessdef_inject_compose; eauto; cycle 1.
-        { eapply memval_inject_incr; eauto. }
-        unfold Mem.alloc in *.
-        clarify.
-        ss.
-        rewrite PMap.gsspec. des_ifs.
-        erewrite <- freed_from_contents; eauto. refl.
-      }
-      clear_tac.
-      eapply memval_inject_incr; eauto.
-      unfold Mem.alloc in *. clarify. ss. unfold Mem.perm in *. ss.
-      rewrite PMap.gsspec in *. des_ifs.
-      erewrite Mem.unchanged_on_contents; try apply FREE; eauto.
-      { eapply mi_memval; eauto.
-        eapply freed_from_perm_le; eauto.
-      }
-      { ii; ss. des_ifs. ii.
-        exploit freed_from_noperm; eauto. eauto with mem.
-      }
-      { des_ifs. ii.
-        exploit freed_from_noperm; eauto. eauto with mem.
-      }
-      { apply NNPP. ii. exploit Mem.mi_freeblocks; eauto. i; clarify. }
-  - ii; ss. unfold Mem.valid_block in *. ss.
-    exploit Mem.alloc_result; eauto. i; subst.
-    exploit Mem.nextblock_alloc; eauto. i.
-    des_ifs.
-    + exfalso. eapply H. rewrite H0. xomega.
-    + eapply mi_freeblocks; eauto. ii. eapply H.
-      rewrite H0. erewrite freed_from_nextblock; eauto. xomega.
-  - ii. des_ifs; eauto.
-  - ii. unfold Mem.perm in *. ss.
-    destruct (eq_block b1 blk_new); clarify.
-    { specialize (mi_no_overlap blk_old blk_tgt delta b2 b2' delta2).
-      des_ifs.
-      destruct (peq b2 blk_old).
-      { clarify. right. ii.
-        exploit Mem.perm_alloc_3; eauto. i.
-        hexploit freed_from_noperm; eauto. i. specialize (H5 ofs1 H4).
-        exploit Mem.perm_alloc_4; eauto. i.
-        assert(ofs1 = ofs2) by xomega. clarify.
-      }
-      eapply mi_no_overlap; eauto.
-      - exploit Mem.perm_alloc_3; eauto. i.
-        eapply Mem.perm_cur_max. eapply Mem.perm_implies with Freeable; (eauto with mem).
-        eapply freed_from_perm; eauto.
-      - assert(Mem.perm_order' ((Mem.mem_access m_src1) !! b2 ofs2 Max) Nonempty).
-        { eapply Mem.perm_alloc_4; eauto. }
-        inv FREE.
-        eapply Mem.unchanged_on_perm; eauto.
-        { ss. des_ifs. }
-        { apply NNPP. ii. exploit Mem.mi_freeblocks; eauto. i; clarify. }
-    }
-    destruct (eq_block b2 blk_new); clarify.
-    {
-      specialize (mi_no_overlap b1 b1' delta1 blk_old blk_tgt delta).
-      destruct (peq b1 blk_old).
-      { clarify. right. ii.
-        exploit Mem.perm_alloc_3; eauto. i.
-        hexploit freed_from_noperm; eauto. i. specialize (H5 ofs2 H4).
-        exploit Mem.perm_alloc_4; try apply H2; eauto. i.
-        assert(ofs1 = ofs2) by xomega. clarify.
-      }
-      eapply mi_no_overlap; eauto.
-      - assert(Mem.perm_order' ((Mem.mem_access m_src1) !! b1 ofs1 Max) Nonempty).
-        { eapply Mem.perm_alloc_4; eauto. }
-        inv FREE.
-        eapply Mem.unchanged_on_perm; eauto.
-        { ss. des_ifs. }
-        { apply NNPP. ii. exploit Mem.mi_freeblocks; eauto. i; clarify. }
-      - exploit Mem.perm_alloc_3; eauto. i.
-        eapply Mem.perm_cur_max. eapply Mem.perm_implies with Freeable; (eauto with mem).
-        eapply freed_from_perm; eauto.
-    }
-    specialize (mi_no_overlap b1 b1' delta1 b2 b2' delta2).
-    eapply mi_no_overlap; eauto.
-    + assert(Mem.perm m_src1 b1 ofs1 Max Nonempty).
-      { eapply Mem.perm_alloc_4; eauto. }
-      eapply freed_from_perm_le; eauto.
-    + assert(Mem.perm m_src1 b2 ofs2 Max Nonempty).
-      { eapply Mem.perm_alloc_4; eauto. }
-      eapply freed_from_perm_le; eauto.
-  - ii. ss. dup FREE. inv FREE. inv freed_from_unchanged0.
-    assert (Mem.perm m_src2 b (Ptrofs.unsigned ofs) Max Nonempty \/
-            Mem.perm m_src2 b (Ptrofs.unsigned ofs - 1) Max Nonempty).
-    { eauto. } clear H0. des_ifs.
-    + eapply mi_representable; eauto.
-      des.
-      * left. exploit freed_from_perm0.
-        { eapply Mem.perm_alloc_3; eauto. }
-        i. eapply Mem.perm_cur_max. eapply Mem.perm_implies; eauto. econs.
-      * right. exploit freed_from_perm0.
-        { eapply Mem.perm_alloc_3; eauto. }
-        i. eapply Mem.perm_cur_max. eapply Mem.perm_implies; eauto. econs.
-    + eapply mi_representable; eauto.
-      assert (Mem.perm m_src1 b (Ptrofs.unsigned ofs) Max Nonempty \/
-              Mem.perm m_src1 b (Ptrofs.unsigned ofs - 1) Max Nonempty).
-      { des; eapply Mem.perm_alloc_4 in H1; eauto. } clear H1.
-      des; [left|right]; eapply freed_from_perm_greater; eauto.
-  - unfold Mem.perm. ss.
-    ii. des_ifs.
-    + destruct (classic (lo <= ofs < hi)).
-      { left. eapply Mem.perm_cur. eapply Mem.perm_implies with Freeable; eauto with mem. }
-      { right. ii. exploit Mem.perm_alloc_3; eauto. }
-    + exploit mi_perm_inv; eauto. i.
-      unfold Mem.alloc in *. clarify. ss. rewrite PMap.gsspec. des_ifs.
-      destruct (classic (b1 = blk_old /\ lo <= ofs < hi)).
-      { des_safe; clarify. right. eapply freed_from_noperm; eauto. }
-      { apply not_and_or in H2.
-        destruct H2.
-        - des; ss.
-          + left. inv FREE.
-            eapply Mem.unchanged_on_perm with (m_after := m_src1) (m_before := m_src0); eauto.
-            { ii; ss. des_ifs. }
-            { apply NNPP. ii. exploit Mem.mi_freeblocks; eauto. i; clarify. }
-          + right. ii. eapply H1. eapply freed_from_perm_le; eauto.
-        - des; ss.
-          + left. inv FREE.
-            eapply Mem.unchanged_on_perm with (m_after := m_src1) (m_before := m_src0); eauto.
-            { ii; ss. des_ifs. }
-            { apply NNPP. ii. exploit Mem.mi_freeblocks; eauto. i; clarify. }
-          + right. ii. eapply H1. eapply freed_from_perm_le; eauto.
-      }
-Qed.
-Local Opaque Mem.alloc.
-
-Lemma free_freed_from m0 m1 blk lo hi
-      (FREE: Mem.free m0 blk lo hi = Some m1)
-  :
-    freed_from m0 m1 blk lo hi.
-Proof.
-  econs.
-  - eapply Mem.free_unchanged_on; eauto.
-    i. des_ifs.
-  - eapply Mem.nextblock_free; eauto.
-  - eapply Mem.free_range_perm; eauto.
-  - eapply Mem_free_noperm; eauto.
-  - i. Local Transparent Mem.free. unfold Mem.free in *.
-    des_ifs.
-Qed.
-
-Lemma init_mem_freed_from m_init
-  :
-    freed_from m_init m_init 1%positive 0 0.
-Proof.
-  econs; ii; auto; try omega.
-  econs; eauto. refl.
-Qed.
-
-Inductive inj_same (j: meminj) v_caller v_callee : Prop :=
-| inj_same_intro
-    blk_caller blk_callee blk delta ofs
-    (OFSZERO: ofs = Ptrofs.zero)
-    (CALLERRSP: v_caller = Vptr blk_caller ofs true)
-    (CALLEERSP: v_callee = Vptr blk_callee ofs true)
-    (CALLER: j blk_caller = Some (blk, delta))
-    (CALLEE: j blk_callee = Some (blk, delta)).
-
-Lemma inj_same_inj j v_caller v_callee v_tgt
-      (SAME: inj_same j v_caller v_callee)
-      (INJ: Val.inject j v_caller v_tgt)
-  :
-    Val.inject j v_callee v_tgt.
-Proof.
-  inv SAME. inv INJ. clarify. econs; eauto.
-Qed.
-
-Lemma inj_same_inj2 j v_caller v_callee v_tgt
-      (SAME: inj_same j v_caller v_callee)
-      (INJ: Val.inject j v_callee v_tgt)
-  :
-    Val.inject j v_caller v_tgt.
-Proof.
-  inv SAME. inv INJ. clarify. econs; eauto.
-Qed.
-
-Definition to_fake (v: val) : val :=
-  match v with
-  | Vptr blk ofs true => Vptr blk ofs false
-  | _ => v
-  end.
-
-Lemma to_fake_inj j v_src v_tgt
-      (INJ: Val.inject j v_src v_tgt)
-  :
-    Val.inject j (to_fake v_src) v_tgt.
-Proof. unfold to_fake. inv INJ; econs; eauto. Qed.
-
-Lemma to_fake_inj2 j v_src v_tgt
-      (INJ: Val.inject j (to_fake v_src) v_tgt)
-  :
-    Val.inject j v_src v_tgt.
-Proof. unfold to_fake in *. des_ifs; inv INJ; clarify. econs; eauto. Qed.
 
 Lemma unfree_free_inj_inj_wf P j (m_src0 m_src1 m_src2 m_tgt: mem)
       blk0 blk1 delta1 delta2 ofs1 ofs2 size
@@ -651,300 +481,51 @@ Lemma unfree_free_inj_inj_wf P j (m_src0 m_src1 m_src2 m_tgt: mem)
       (DELTA2: delta2 = Ptrofs.unsigned ofs2)
       (FREE: Mem.free m_src0 blk0 delta1 (delta1 + size) = Some m_src1)
       (UNFREE: Mem_unfree m_src1 blk1 delta2 (delta2 + size) = Some m_src2)
-      (SAME: inj_same j (Vptr blk1 ofs2 true) (Vptr blk0 ofs1 true))
+      (SYMB: skenv_inject ge j m_src0)
+      (SAME: inj_same j (Vptr blk1 ofs2) (Vptr blk0 ofs1))
+      (MAPPED: j blk1 <> None)
       (INJ: Mem.inject j m_src0 m_tgt)
       (WFINJ: inj_range_wf j m_src0 P)
       (RANGE: range delta2 (delta2 + size) <1= P blk1)
   :
-    <<INJ: Mem.inject j m_src2 m_tgt>> /\ <<WFINJ: inj_range_wf j m_src2 P>>.
+    (<<INJ: Mem.inject j m_src2 m_tgt>>) /\
+    (<<WFINJ: inj_range_wf j m_src2 P>>) /\
+    (<<SYMB: skenv_inject ge j m_src2>>)
+.
 Proof.
-  inv SAME. clarify. des_ifs. eapply private_unfree_inj_inj_wf; cycle 4; eauto.
-  - ii. destruct (WFINJ blk0).
-    + econs 1; eauto.
+  subst. destruct (j blk1) as [[]|] eqn:BEQ; clarify; cycle 1.
+  assert (SAME0: j blk0 = Some (b, z - Ptrofs.unsigned ofs1 + Ptrofs.unsigned ofs2)).
+  { inv SAME.
+    - inv VAL0. inv VAL1. rewrite BEQ in *. inv INJ0. rewrite INJ1.
+      repeat f_equal. lia.
+    - inv EQ. rewrite BEQ. repeat f_equal. lia.
+  }
+  eapply private_unfree_inj_inj_wf; cycle 4; eauto.
+  - eapply skenv_inject_max_perm; eauto.
+    i. eapply Mem.perm_free_3; eauto.
+  - ii. destruct (WFINJ blk).
+    +  econs 1; eauto.
     + econs 2; eauto.
       i. eapply ALIGN. ii. eapply H in PR. des; eauto.
       left. eapply Mem.perm_free_3; eauto.
   - eapply Mem.free_left_inject; eauto.
-  - rewrite Z.add_comm.
-    replace (delta + (Ptrofs.unsigned Ptrofs.zero + size)) with ((Ptrofs.unsigned Ptrofs.zero + size)+delta) by lia.
-    eapply Mem.range_perm_inj; try apply INJ; eauto.
-    eapply Mem.free_range_perm; eauto.
+  - hexploit Mem.free_range_perm; eauto. i.
+    eapply Mem.range_perm_inj in H; try apply INJ; eauto.
+    replace (z + Ptrofs.unsigned ofs2) with
+        (Ptrofs.unsigned ofs1 + (z - Ptrofs.unsigned ofs1 + Ptrofs.unsigned ofs2)); [|lia].
+    replace (z + (Ptrofs.unsigned ofs2 + size)) with
+        (Ptrofs.unsigned ofs1 + size + (z - Ptrofs.unsigned ofs1 + Ptrofs.unsigned ofs2)); [|lia].
+    auto.
   - intros delta' RANGE0 blk' ofs' INJECT. unfold range in *.
-    destruct (eq_block blk' blk_callee); clarify.
+    destruct (eq_block blk' blk0); clarify.
     + eapply Mem.perm_free_2; eauto. lia.
     + intros PERM. eapply Mem.perm_free_3 in PERM; eauto.
       eapply Mem.free_range_perm in FREE.
       exploit Mem.inject_no_overlap; eauto.
-      eapply Mem.perm_max; eauto.
-      eapply Mem.perm_implies; eauto.
-      eapply FREE; eauto.
-      * assert (Ptrofs.unsigned Ptrofs.zero <= delta' - delta < Ptrofs.unsigned Ptrofs.zero + size).
-        rewrite Ptrofs.unsigned_zero in *. lia. eauto.
-      * econs.
-      * splits. des; eauto. lia.
+      * eapply Mem.perm_max; eauto.
+        eapply Mem.perm_implies; try eapply FREE; [|econs].
+        instantiate (1:=delta' - z + Ptrofs.unsigned ofs1 - Ptrofs.unsigned ofs2). lia.
+      * ii. des; clarify. zsimpl. lia.
 Qed.
 
-Lemma memcpy_load
-      m_src0 m_src1 m_src2 chunk blk_old blk_new lo hi ofs v
-      (NEQ: blk_old <> blk_new)
-      (FREE: freed_from m_src0 m_src1 blk_old lo hi)
-      (ALLOC: Mem.alloc m_src1 lo hi = (m_src2, blk_new))
-      (BOUND0: lo <= ofs)
-      (BOUND1: ofs + size_chunk chunk <= hi)
-      (LOAD: Mem.load chunk m_src0 blk_old ofs = Some v)
-  :
-    Mem.load chunk (memcpy m_src2 blk_old blk_new)
-             blk_new ofs = Some v.
-Proof.
-  Local Transparent Mem.load. unfold Mem.load in *. des_ifs.
-  - f_equal. f_equal. ss. rewrite PMap.gss.
-    rewrite size_chunk_conv in *.
-    generalize (size_chunk_nat chunk) ofs BOUND0 BOUND1.
-    induction n; ss.
-    i. f_equal.
-    + symmetry. erewrite freed_from_contents; [|apply FREE|lia].
-      f_equal. rewrite (Mem.alloc_result _ _ _ _ _ ALLOC) in NEQ.
-      Local Transparent Mem.alloc. unfold Mem.alloc in *.
-      clarify. ss. symmetry. apply PMap.gso; auto.
-    + eapply IHn; lia.
-  - exfalso. eapply n. unfold Mem.valid_access in *. des. split; auto.
-    ii. eapply Mem.perm_implies; [|econs 2].
-    exploit Mem.perm_alloc_2; eauto. lia.
-Qed.
-
-Lemma nextblock_unvalid CTX j m1 m2
-      (INJ: @Mem.inject CTX j m1 m2)
-  :
-    j (Mem.nextblock m1) = None.
-Proof.
-  inv INJ. eapply mi_freeblocks.
-  unfold Mem.valid_block. apply Plt_strict.
-Qed.
-
-Inductive almost_eq : val -> val -> Prop :=
-| almost_eq_refl v : almost_eq v v
-| almost_eq_ptr blk ofs b1 b2 : almost_eq (Vptr blk ofs b1) (Vptr blk ofs b2)
-.
-
-Lemma to_fake_almost_eq v
-  :
-    almost_eq v (to_fake v).
-Proof.
-  destruct v; try econs. destruct b0; econs.
-Qed.
-
-Lemma almost_eq_commute j v_src0 v_src1 v_tgt
-      (INJ: Val.inject j v_src1 v_tgt)
-      (EQ: almost_eq v_src0 v_src1)
-  :
-    Val.inject j v_src0 v_tgt.
-Proof.
-  inv EQ; eauto.
-  destruct b1, b2; inv INJ; try econs; eauto. clarify.
-Qed.
-
-Lemma lessdef_commute j v_src0 v_src1 v_tgt
-      (INJ: Val.inject j v_src1 v_tgt)
-      (LESS: Val.lessdef v_src0 v_src1)
-  :
-    Val.inject j v_src0 v_tgt.
-Proof.
-  inv LESS; inv INJ; eauto.
-Qed.
-
-Lemma to_fake_fake_ptr v : ~ is_real_ptr (to_fake v).
-Proof.
-  intros i. inv i. destruct v; ss. destruct b0; ss.
-Qed.
-
-Lemma callee_injection_incr j old_blk new_blk
-      (INJ_NONE: j new_blk = None)
-  :
-    inject_incr j (callee_injection j old_blk new_blk).
-Proof.
-  unfold callee_injection. ii. des_ifs.
-Qed.
-
-Definition extcall_args_reg (mr: mreg) (sg: signature):
-  {In (R mr) (regs_of_rpairs (loc_arguments sg))} +
-  {~ In (R mr) (regs_of_rpairs (loc_arguments sg))}.
-Proof.
-  generalize (regs_of_rpairs (loc_arguments sg)). induction l.
-  - ss. tauto.
-  - ss. inv IHl; [tauto|].
-    destruct a.
-    + destruct (mreg_eq r mr); [clarify; eauto|].
-      right. intros []; clarify.
-    + right. intros []; clarify.
-Qed.
-
-Definition src_init_rs sg (rs_src: regset) (rsp: val) : regset :=
-  fun (pr : PregEq.t) =>
-    match Asm.to_mreg pr with
-    | Some mr =>
-      if (extcall_args_reg mr sg)
-      then (rs_src pr)
-      else (to_fake (rs_src pr))
-    | None =>
-      match pr with
-      | IR RSP => rsp
-      | PC => rs_src PC
-      | RA => to_fake (rs_src RA)
-      | _ => to_fake (rs_src pr)
-      end
-    end.
-
-Program Definition arg_copy_mem (m: mem) (blk_old blk_new: Values.block)
-        (sg: signature) (args: list val) : mem :=
-  Mem.mkmem
-    (admit "")
-    m.(Mem.mem_access) m.(Mem.nextblock)
-                           m.(Mem.access_max) m.(Mem.nextblock_noaccess)
-                                                  _.
-Next Obligation.
-Admitted.
-
-Definition arg_copy_reg (sg: signature) (args: list val)
-           (rs: regset) : regset.
-Admitted.
-
-Lemma arg_copy_reg_spec sg args rs pr
-      (DIFF: (arg_copy_reg sg args rs) pr <> rs pr)
-  :
-    (<<UNDEF: (arg_copy_reg sg args rs) pr = Vundef>>) /\
-    (<<ARGS: exists mr (MR: to_mreg pr = Some mr),
-        In (R mr) (regs_of_rpairs (loc_arguments sg))>>).
-Admitted.
-
-Lemma arg_copy_reg_RA sg args rs
-  :
-    (arg_copy_reg sg args rs) RA = rs RA.
-Proof.
-  destruct (classic (arg_copy_reg sg args rs RA = rs RA)); eauto.
-  exploit arg_copy_reg_spec; eauto. i. des.
-  clarify.
-Qed.
-
-Lemma arg_copy_reg_PC sg args rs
-  :
-    (arg_copy_reg sg args rs) PC = rs PC.
-Proof.
-  destruct (classic (arg_copy_reg sg args rs PC = rs PC)); eauto.
-  exploit arg_copy_reg_spec; eauto. i. des.
-  clarify.
-Qed.
-
-Lemma arg_copy_reg_RSP sg args rs
-  :
-    (arg_copy_reg sg args rs) RSP = rs RSP.
-Proof.
-  destruct (classic (arg_copy_reg sg args rs RSP = rs RSP)); eauto.
-  exploit arg_copy_reg_spec; eauto. i. des.
-  clarify.
-Qed.
-
-Lemma arg_copy_reg_more_undef sg args rs pr
-  :
-    (arg_copy_reg sg args rs) pr = rs pr \/
-    (arg_copy_reg sg args rs) pr = Vundef.
-Proof.
-  destruct (classic (arg_copy_reg sg args rs pr = rs pr)); eauto.
-  exploit arg_copy_reg_spec; eauto. i. des.
-  eauto.
-Qed.
-
-Lemma arg_copy_reg_callee_save sg args rs mr
-      (SAVE: is_callee_save mr)
-  :
-    (arg_copy_reg sg args rs) (to_preg mr) = rs (to_preg mr).
-Proof.
-  destruct (classic (arg_copy_reg sg args rs (to_preg mr) = rs (to_preg mr))); eauto.
-  exploit arg_copy_reg_spec; eauto. i. des.
-  rewrite to_preg_to_mreg in MR. clarify.
-  exploit loc_args_callee_save_disjoint; eauto.
-  intros [].
-Qed.
-
-Lemma memcpy_store_arguments
-      rs m_src0 m_src1 m_src2 sg args blk_old blk_new ofs
-      (ARGS: Asm.extcall_arguments rs m_src0 sg args)
-      (RSRSP: rs RSP = Vptr blk_old ofs true)
-      (OFSZERO: ofs = Ptrofs.zero)
-      (NEQ: blk_old <> blk_new)
-      (SZ: 4 * size_arguments sg <= Ptrofs.max_unsigned)
-      (FREE: freed_from m_src0 m_src1
-                        blk_old ofs.(Ptrofs.unsigned)
-                                      (ofs.(Ptrofs.unsigned)+4*size_arguments sg))
-      (ALLOC: Mem.alloc m_src1 ofs.(Ptrofs.unsigned)
-                                     (ofs.(Ptrofs.unsigned)+4*size_arguments sg)
-              = (m_src2, blk_new))
-  :
-    store_arguments
-      m_src1
-      (arg_copy_reg sg args (src_init_rs sg rs (Vptr blk_new ofs true)))
-      (typify_list args (sig_args sg))
-      sg (arg_copy_mem m_src2 blk_old blk_new sg args).
-Proof.
-Admitted.
-
-Lemma arg_copy_mem_extends m blk_old blk_new sg args
-  :
-    Mem.extends (arg_copy_mem m blk_old blk_new sg args) (memcpy m blk_old blk_new).
-Proof.
-Admitted.
-
-
-(* Lemma memcpy_store_arguments *)
-(*       rs m_src0 m_src1 m_src2 sg args blk_old blk_new ofs *)
-(*       (ARGS: Asm.extcall_arguments rs m_src0 sg args) *)
-(*       (RSRSP: rs # RSP = Vptr blk_old ofs true) *)
-(*       (OFSZERO: ofs = Ptrofs.zero) *)
-(*       (NEQ: blk_old <> blk_new) *)
-(*       (SZ: 4 * size_arguments sg <= Ptrofs.max_unsigned) *)
-(*       (FREE: freed_from m_src0 m_src1 *)
-(*                         blk_old ofs.(Ptrofs.unsigned) *)
-(*                                       (ofs.(Ptrofs.unsigned)+4*size_arguments sg)) *)
-(*       (ALLOC: Mem.alloc m_src1 ofs.(Ptrofs.unsigned) *)
-(*                                      (ofs.(Ptrofs.unsigned)+4*size_arguments sg) *)
-(*               = (m_src2, blk_new)) *)
-(*   : *)
-(*     store_arguments *)
-(*       m_src1 *)
-(*       (src_init_rs sg rs (Vptr blk_new ofs true)) *)
-(*       args sg (memcpy m_src2 blk_old blk_new). *)
-(* Proof. *)
-(*   admit "it doesn't hold.". *)
-(* Qed. *)
-
-(*   clarify; econs; eauto. *)
-(*   - unfold extcall_arguments in *. *)
-(*     revert args ARGS. generalize (is_tail_refl (loc_arguments sg)). *)
-(*     assert (forall *)
-(*                l args *)
-(*                (TAIL: is_tail l (loc_arguments sg)) *)
-(*                (ARGS: list_forall2 (extcall_arg_pair rs m_src0) l args) *)
-(*              , *)
-(*                list_forall2 *)
-(*                  (extcall_arg_pair (src_init_rs sg rs (Vptr blk_new Ptrofs.zero true)) *)
-(*                                    (memcpy m_src2 blk_old blk_new)) l args); auto. *)
-(*     induction l; i; inv ARGS; econs; eauto. *)
-(*     + inv H1; econs. *)
-(*       * eapply init_argument; eauto. *)
-(*         apply tail_In with (a := One l0) in TAIL; [|econs; eauto]. *)
-(*         eapply regs_of_rpair_In in TAIL. auto. *)
-(*       * eapply init_argument; eauto. *)
-(*         apply tail_In with (a := Twolong hi lo) in TAIL; [|econs; eauto]. *)
-(*         eapply regs_of_rpair_In in TAIL. tauto. *)
-(*       * eapply init_argument; eauto. *)
-(*         apply tail_In with (a := Twolong hi lo) in TAIL; [|econs; eauto]. *)
-(*         eapply regs_of_rpair_In in TAIL. tauto. *)
-(*     + eapply IHl; auto. *)
-(*       eapply is_tail_trans; eauto. econs 2. econs 1. *)
-(*   - econs; ss; eauto. *)
-(*     + refl. *)
-(*     + intros b ofs0 IN PERM. des_ifs. *)
-(*       * exfalso. apply IN. eapply Mem.perm_alloc_3; eauto. *)
-(*       * f_equal. eapply PMap.gso; auto. *)
-(*   - ss. ii. unfold Mem.perm. ss. *)
-(*     eapply Mem.perm_alloc_2; eauto. *)
-(* Qed. *)
+End INJRANGEWF.
